start resolving remaining sorrys, move well-formed total consistency to TotalSemantics.thy

TotalSemantics.thy
@@ -575,6 +575,87 @@ proof -
     by auto
 qed
 
+subsection \<open>Well-formed state consistency\<close>
+
+text \<open>Many of the theorems are parametrized by the state consistency. Many of the theorems require
+certain properties on the state consistency. The following well-formedness definition captures
+these properties.\<close>
+
+definition wf_total_consistency 
+  where "wf_total_consistency ctxt R Rt \<equiv> 
+               mono_prop_downward R \<and>
+               (\<forall>\<omega>. is_empty_total_full \<omega> \<longrightarrow> R \<omega>) \<and>
+               (\<forall>\<omega> \<omega>' \<Lambda> stmt. R \<omega> \<longrightarrow> red_stmt_total ctxt R \<Lambda> stmt \<omega> (RNormal \<omega>') \<longrightarrow> R \<omega>') \<and>
+               \<comment>\<open>The following statement ensures that states in the body of a scope preserve consistency.\<close>
+               (\<forall>\<omega> v. R \<omega> \<longrightarrow> R (shift_and_add_state_total \<omega> v)) \<and> 
+               (\<forall>\<omega>. R \<omega> \<longleftrightarrow> (Rt (get_total_full \<omega>) \<and> (\<forall>lbl \<phi>. get_trace_total \<omega> lbl = Some \<phi> \<longrightarrow> Rt \<phi>)) )"
+
+lemma total_consistencyI:
+  assumes "wf_total_consistency ctxt R Rt"
+      and "Rt (get_total_full \<omega>)"
+      and "\<And> lbl \<phi>. get_trace_total \<omega> lbl = Some \<phi> \<Longrightarrow> Rt \<phi>"
+    shows "R \<omega>"
+  using assms
+  unfolding wf_total_consistency_def
+  by blast
+
+lemma wf_total_consistency_trivial: "wf_total_consistency ctxt (\<lambda>_.True) (\<lambda>_.True)"
+  unfolding wf_total_consistency_def mono_prop_downward_def
+  by blast
+
+lemma total_consistency_red_stmt_preserve:
+  assumes "wf_total_consistency ctxt R Rt" 
+      and "R \<omega>"
+      and "red_stmt_total ctxt R \<Lambda> stmt \<omega> (RNormal \<omega>')"
+    shows "R \<omega>'"
+  using assms
+  unfolding wf_total_consistency_def
+  by blast
+
+lemma total_consistency_store_update:
+  assumes "wf_total_consistency ctxt R Rt" 
+      and "R \<omega>" 
+      and "get_total_full \<omega>' = get_total_full \<omega>" 
+      and "get_trace_total \<omega>' = get_trace_total \<omega>"
+    shows "R \<omega>'"
+  using assms
+  unfolding wf_total_consistency_def
+  by metis
+
+lemma total_consistency_store_update_2:
+  assumes "wf_total_consistency ctxt R Rt" 
+      and "R \<omega>" 
+    shows "R (\<omega> \<lparr> get_store_total := \<sigma> \<rparr>)"
+  using assms total_consistency_store_update
+  by fastforce
+
+lemma total_consistency_trace_update:
+  assumes "wf_total_consistency ctxt R Rt" 
+      and "R \<omega>" 
+      and "get_store_total \<omega>' = get_store_total \<omega>"
+      and "get_total_full \<omega>' = get_total_full \<omega>" 
+      and "\<And> lbl \<phi>. get_trace_total \<omega>' lbl = Some \<phi> \<Longrightarrow> Rt \<phi>"
+    shows "R \<omega>'"
+  using assms 
+  unfolding wf_total_consistency_def
+  by simp
+
+lemma total_consistency_trace_update_2:
+  assumes "wf_total_consistency ctxt R Rt" 
+      and "R \<omega>" 
+      and "\<And> lbl \<phi>. t lbl = Some \<phi> \<Longrightarrow> Rt \<phi>"
+    shows "R (\<omega> \<lparr> get_trace_total := t \<rparr>)"
+  using assms 
+  unfolding wf_total_consistency_def
+  by simp
+
+lemma wf_total_consistency_trace_mono_downwardD:
+  assumes "wf_total_consistency ctxt R Rt"
+  shows "mono_prop_downward R"
+  using assms
+  unfolding wf_total_consistency_def
+  by blast
+
 subsection \<open>Experimental definitions\<close>
 
 definition assertion_sat :: "'a total_context \<Rightarrow> ('a full_total_state \<Rightarrow> bool) \<Rightarrow> type_context \<Rightarrow> assertion \<Rightarrow> 'a full_total_state \<Rightarrow> bool"
